Refactor to use iris cmras

src/ra/IPM.v
@@ -3,10 +3,10 @@ From Fairness Require Import PCM ITreeLib IProp.
 
 Set Implicit Arguments.
 
-From iris.bi Require Import derived_connectives updates.
+From iris.bi Require Import derived_connectives derived_laws updates.
 From iris.prelude Require Import options.
 From iris.proofmode Require Export tactics.
-From Fairness Require Export DisableSsreflect.
+From iris.algebra Require Import cmra updates proofmode_classes.
 Arguments Z.of_nat: simpl nomatch.
 
 Require Import Program.
@@ -15,8 +15,8 @@ Section IPM.
   Context {Σ: GRA.t}.
 
   (* Trivial Ofe Structure *)
-  Inductive uPred_equiv' (P Q : iProp') : Prop :=
-    { uPred_in_equiv : ∀ x, URA.wf x -> P x <-> Q x }.
+  Inductive uPred_equiv' (P Q : (@iProp' Σ)) : Prop :=
+    { uPred_in_equiv : ∀ x, ✓ x -> P x <-> Q x }.
 
   Local Instance uPred_equiv : Equiv iProp' := uPred_equiv'.
   Definition uPred_dist' (n : nat) (P Q : iProp') : Prop := uPred_equiv' P Q.
@@ -95,25 +95,25 @@ Section IPM.
       { uipropall. ii. inv H1. exploit H; eauto. i. eexists. eapply x3; eauto. }
     - econs. i. split.
       { uipropall. ii. inv H2. des. subst. eexists. esplits; eauto.
-        { eapply H; eauto. eapply URA.wf_mon; eauto. }
-        { eapply H0; eauto. eapply URA.wf_mon; eauto. rewrite URA.add_comm. eauto. }
+        { eapply H; eauto. eapply cmra_valid_op_l. rewrite H3 in H1. eauto. }
+        { eapply H0; eauto. eapply cmra_valid_op_r. rewrite H3 in H1. eauto. }
       }
       { uipropall. ii. inv H2. des. subst. eexists. esplits; eauto.
-        { eapply H; eauto. eapply URA.wf_mon; eauto. }
-        { eapply H0; eauto. eapply URA.wf_mon; eauto. rewrite URA.add_comm. eauto. }
+        { eapply H; eauto. eapply cmra_valid_op_l. rewrite H3 in H1. eauto. }
+        { eapply H0; eauto. eapply cmra_valid_op_r. rewrite H3 in H1. eauto. }
       }
     - econs. uipropall. i. split.
       { ii. exploit H2; eauto.
-        { eapply H; eauto. eapply URA.wf_mon; eauto. rewrite URA.add_comm. eauto. }
+        { eapply H; eauto. eapply cmra_valid_op_r. eauto. }
         { i. eapply H0; eauto. }
       }
       { ii. exploit H2; eauto.
-        { eapply H; eauto. eapply URA.wf_mon; eauto. rewrite URA.add_comm. eauto. }
+        { eapply H; eauto. eapply cmra_valid_op_r. eauto. }
         { i. eapply H0; eauto. }
       }
     - ii. econs. uipropall. i. split.
-      { ii. eapply H; ss. eapply URA.wf_core. auto. }
-      { ii. eapply H; ss. eapply URA.wf_core. auto. }
+      { ii. eapply H; ss. apply cmra_core_valid. auto. }
+      { ii. eapply H; ss. apply cmra_core_valid. auto. }
     - exact Pure_intro.
     - exact Pure_elim.
     - exact And_elim_l.
@@ -158,7 +158,7 @@ Section IPM.
     {| bi_bi_mixin := iProp_bi_mixin;
        bi_bi_later_mixin := iProp_bi_later_mixin |}.
 
-  Definition OwnM (M: URA.t) `{@GRA.inG M Σ} (r: M): iProp := Own (GRA.embed r).
+  Definition OwnM (M: ucmra) `{@GRA.inG M Σ} (r: M): iProp := Own (GRA.embed r).
 
   (** extra BI instances *)
   Lemma iProp_bupd_mixin: BiBUpdMixin iProp Upd.
@@ -166,9 +166,9 @@ Section IPM.
     econs.
     - ii. econs. unfold bupd. uipropall. i. split.
       { ii. exploit H1; eauto. i. des. esplits; eauto.
-        eapply H; eauto. eapply URA.wf_mon; eauto. }
+        eapply H; eauto. eapply cmra_valid_op_l. eauto. }
       { ii. exploit H1; eauto. i. des. esplits; eauto.
-        eapply H; eauto. eapply URA.wf_mon; eauto. }
+        eapply H; eauto. eapply cmra_valid_op_l. eauto. }
     - exact Upd_intro.
     - exact Upd_mono.
     - exact Upd_trans.
@@ -179,7 +179,8 @@ Section IPM.
   Global Instance iProp_absorbing (P: iProp): Absorbing P.
   Proof.
     rr. uipropall. i. rr in H. uipropall. des. eapply iProp_mono; eauto.
-    exists a. rewrite H. r_solve.
+    eapply iProp_mono; [done| |exact H1].
+    exists a. rewrite H. by rewrite (comm op).
   Qed.
 
   Global Instance iProp_affine (P: iProp): Affine P.
@@ -214,11 +215,14 @@ Section IPM.
   Qed.
 
 End IPM.
+Global Arguments iProp : clear implicits.
+
 Global Hint Immediate iProp_bi_affine : core.
 Arguments OwnM: simpl never.
 
 Section TEST.
   Context {Σ: GRA.t}.
+  Notation iProp := (iProp Σ).
 
   Goal forall (P Q R: iProp) (PQ: P -∗ Q) (QR: Q -∗ R), P -∗ R.
   Proof.
@@ -233,11 +237,11 @@ Section TEST.
   Qed.
 End TEST.
 
-Infix "⊢" := (@bi_entails iProp).
-Notation "#=> P" := ((@bupd (bi_car iProp) (@bi_bupd_bupd iProp iProp_bi_bupd)) P) (at level 99).
+Notation "#=> P" := ((@bupd (bi_car (iProp _)) (@bi_bupd_bupd (iProp _) iProp_bi_bupd)) P) (at level 99).
 
 Section IUPD.
   Context {Σ: GRA.t}.
+  Notation iProp := (iProp Σ).
 
   Definition IUpd (I: iProp): iProp -> iProp :=
     fun P => (I -∗ #=> (I ∗ P))%I.
@@ -284,160 +288,134 @@ Section IUPD.
   Qed.
   Global Instance iProp_bi_bupd_IUpd I: BiBUpd iProp := {| bi_bupd_mixin := iProp_bupd_mixin_IUpd I |}.
 End IUPD.
-Notation "#=( Q )=> P" := ((@bupd (bi_car iProp) (@bi_bupd_bupd iProp (iProp_bi_bupd_IUpd Q))) P) (at level 99).
+Notation "#=( Q )=> P" := ((@bupd (bi_car (iProp _)) (@bi_bupd_bupd (iProp _) (iProp_bi_bupd_IUpd Q))) P) (at level 99).
 Notation "P =( I ) =∗ Q" := (P ⊢ #=( I )=> Q) (only parsing, at level 99) : stdpp_scope.
 Notation "P =( I )=∗ Q" := (P -∗ #=( I )=> Q)%I (at level 99): bi_scope.
-
-
-Class IsOp {A : URA.t} (a b1 b2 : A) := is_op : a = b1 ⋅ b2.
-Global Arguments is_op {_} _ _ _ {_}.
-Global Hint Mode IsOp + - - - : typeclass_instances.
-
-Global Instance is_op_op {A : URA.t} (a b : A) : IsOp (URA.add a b) a b | 100.
-Proof. by rewrite /IsOp. Qed.
-
-Class IsOp' {A : URA.t} (a b1 b2 : A) := is_op' :> IsOp a b1 b2.
-Global Hint Mode IsOp' + ! - - : typeclass_instances.
-Global Hint Mode IsOp' + - ! ! : typeclass_instances.
-
-Class IsOp'LR {A : URA.t} (a b1 b2 : A) := is_op_lr : IsOp a b1 b2.
-Existing Instance is_op_lr | 0.
-Global Hint Mode IsOp'LR + ! - - : typeclass_instances.
-Global Instance is_op_lr_op {A : URA.t} (a b : A) : IsOp'LR (URA.add a b) a b | 0.
-Proof. by rewrite /IsOp'LR /IsOp. Qed.
 
 #[export] Hint Unfold bi_entails bi_sep bi_and bi_or bi_wand bupd bi_bupd_bupd: iprop.
 
 Section class_instances.
   Context `{Σ: GRA.t}.
+  Notation iProp := (iProp Σ).
+
+  Global Instance Own_proper :
+    Proper ((≡) ==> (⊣⊢)) (@Own Σ).
+  Proof.
+    intros x y EQ. uipropall. split. ss. by setoid_rewrite EQ.
+  Qed.
+
+  Lemma Own_op (a1 a2: Σ) :
+    (Own (a1 ⋅ a2)) ⊣⊢ (Own a1 ∗ Own a2).
+  Proof.
+    uipropall. split. simpl. intros x WFx. split.
+    - intros [z ?]; exists (a1), (a2 ⋅ z).
+      split; [by rewrite (assoc op)|].
+      split.
+      + by exists ε; rewrite right_id.
+      + by exists z.
+    - intros (y1&y2&Hx&[z1 Hy1]&[z2 Hy2]); exists (z1 ⋅ z2).
+      by rewrite (assoc op _ z1) -(comm op z1) (assoc op z1)
+          -(assoc op _ a2) (comm op z1) -Hy1 -Hy2.
+  Qed.
+
+  Lemma Own_valid (a : Σ) :
+    Own a -∗ ⌜✓a⌝.
+  Proof.
+    rr. uipropall. i. red. rr. uipropall.
+    by eapply cmra_valid_included; [exact WF|].
+  Qed.
 
   Global Instance from_sep_own (a b1 b2 : Σ) :
     IsOp a b1 b2 →
     FromSep (Own a) (Own b1) (Own b2).
-  Proof.
-    ii. inv H. red. uipropall. i. des. subst.
-    unfold URA.extends in *. des. subst.
-    exists (URA.add ctx0 ctx). repeat rewrite URA.add_assoc.
-    f_equal. rewrite URA.add_comm. rewrite URA.add_assoc. f_equal.
-    eapply URA.add_comm.
-  Qed.
+  Proof. intros. by rewrite /FromSep -Own_op -is_op. Qed.
 
   Global Instance into_and_own p (a b1 b2 : Σ) :
     IsOp a b1 b2 → IntoAnd p (Own a) (Own b1) (Own b2).
-  Proof.
-    ii. apply bi.intuitionistically_if_mono. inv H.
-    uipropall. i. unfold URA.extends in *. des. subst. split.
-    { exists (URA.add b2 ctx). eapply URA.add_assoc. }
-    { exists (URA.add b1 ctx). rewrite URA.add_assoc.
-      f_equal. eapply URA.add_comm. }
-  Qed.
+  Proof. intros. by rewrite /IntoAnd (is_op a) Own_op bi.sep_and. Qed.
 
   Global Instance into_sep_own (a b1 b2 : Σ) :
     IsOp a b1 b2 → IntoSep (Own a) (Own b1) (Own b2).
-  Proof.
-    ii. red. inv H. uipropall. i.
-    unfold URA.extends in *. des. subst.
-    exists b1, (URA.add b2 ctx). split.
-    { symmetry. eapply URA.add_assoc. }
-    esplits.
-    { eapply URA.unit_id. }
-    { eauto. }
-  Qed.
+  Proof. intros. by rewrite /IntoSep (is_op a) Own_op. Qed.
 
-  Global Instance from_sep_ownM (M: URA.t) `{@GRA.inG M Σ} (a b1 b2 : M) :
+  Lemma OwnM_op (M: ucmra) `{@GRA.inG M Σ} (a1 a2: M) :
+    (OwnM (a1 ⋅ a2)) ⊣⊢ (OwnM a1 ∗ OwnM a2).
+  Proof. by rewrite /OwnM -GRA.embed_add Own_op. Qed.
+
+  Global Instance OwnM_proper (M: ucmra) `{@GRA.inG M Σ} :
+    Proper ((≡) ==> (⊣⊢)) (@OwnM Σ M _).
+  Proof. intros x y EQ. by rewrite /OwnM EQ. Qed.
+
+  Global Instance from_sep_ownM (M: ucmra) `{@GRA.inG M Σ} (a b1 b2 : M) :
     IsOp a b1 b2 →
     FromSep (OwnM a) (OwnM b1) (OwnM b2).
-  Proof.
-    ii. red. unfold OwnM. inv H0.
-    iIntros "[H1 H2]". iCombine "H1 H2" as "H".
-    rewrite GRA.embed_add. iApply "H".
-  Qed.
+  Proof. intros. by rewrite /FromSep -OwnM_op -is_op. Qed.
 
-  Global Instance into_and_ownM (M: URA.t) `{@GRA.inG M Σ} p (a b1 b2 : M) :
+  Global Instance into_and_ownM (M: ucmra) `{@GRA.inG M Σ} p (a b1 b2 : M) :
     IsOp a b1 b2 → IntoAnd p (OwnM a) (OwnM b1) (OwnM b2).
-  Proof.
-    ii. red. apply bi.intuitionistically_if_mono. inv H0.
-    unfold OwnM. rewrite <- GRA.embed_add. iIntros "[H1 H2]". iSplit.
-    { iApply "H1". }
-    { iApply "H2". }
-  Qed.
+  Proof. intros. by rewrite /IntoAnd (is_op a) OwnM_op bi.sep_and. Qed.
 
-  Global Instance into_sep_ownM (M: URA.t) `{@GRA.inG M Σ} (a b1 b2 : M) :
+  Global Instance into_sep_ownM (M: ucmra) `{@GRA.inG M Σ} (a b1 b2 : M) :
     IsOp a b1 b2 → IntoSep (OwnM a) (OwnM b1) (OwnM b2).
-  Proof.
-    ii. red. inv H0. unfold OwnM.
-    rewrite <- GRA.embed_add. iIntros "[H1 H2]". iSplitL "H1"; iFrame.
-  Qed.
+  Proof. intros. by rewrite /IntoSep (is_op a) OwnM_op. Qed.
 End class_instances.
 
 
 
 Section ILEMMAS.
   Context `{Σ: GRA.t}.
+  Notation iProp := (iProp Σ).
 
   Lemma from_semantic (a: Σ) (P: iProp') (SAT: P a)
     :
       Own a ⊢ #=> P.
   Proof.
-    uipropall. ss. i. unfold URA.extends in *. des. subst.
-    uipropall. i. esplits; [|apply SAT]. eapply URA.wf_mon.
-    instantiate (1:=ctx0). replace (a ⋅ ctx ⋅ ctx0) with (a ⋅ ctx0 ⋅ ctx); eauto.
-    repeat rewrite <- URA.add_assoc. f_equal. eapply URA.add_comm.
+    uipropall. ss. i. exists r. split; [done|].
+    eapply iProp_mono; [| |exact SAT]; done.
   Qed.
 
-  Lemma to_semantic (a: Σ) (P: iProp') (SAT: Own a ⊢ P) (WF: URA.wf a)
+  Lemma to_semantic (a: Σ) (P: iProp') (SAT: Own a ⊢ P) (WF: ✓ a)
     :
       P a.
-  Proof.
-    uipropall. eapply SAT; eauto. reflexivity.
-  Qed.
+  Proof. uipropall. eapply SAT; eauto. Qed.
 
-  Lemma OwnM_op (M: URA.t) `{@GRA.inG M Σ} (a1 a2: M) :
-      (OwnM (a1 ⋅ a2)) ⊣⊢ (OwnM a1 ∗ OwnM a2).
+  Lemma OwnM_valid (M: ucmra) `{@GRA.inG M Σ} (m: M):
+    OwnM m -∗ ⌜✓ m⌝.
   Proof.
-    iSplit.
-    - unfold OwnM. rewrite <- GRA.embed_add. iIntros "[$ $]".
-    - iIntros "[H1 H2]". iCombine "H1 H2" as "$".
-  Qed.
-
-  Lemma OwnM_valid (M: URA.t) `{@GRA.inG M Σ} (m: M):
-    OwnM m -∗ ⌜URA.wf m⌝.
-  Proof.
-    rr. uipropall. i. red. rr. unfold OwnM, Own in *. uipropall.
-    unfold URA.extends in *. des. subst.
-    eapply URA.wf_mon in WF. eapply GRA.embed_wf. eauto.
+    iIntros "H". iDestruct (Own_valid with "H") as %WF.
+    iPureIntro. eapply GRA.embed_wf. done.
   Qed.
 
   Lemma Upd_Pure P
     :
-      #=> ⌜P⌝ ⊢ ⌜P⌝.
+      #=> (⌜P⌝ : iProp) ⊢ ⌜P⌝.
   Proof.
     rr. uipropall. i. rr. uipropall.
-    hexploit (H URA.unit).
-    { rewrite URA.unit_id. eauto. }
+    hexploit (H ε).
+    { by rewrite right_id. }
     i. des. rr in H1. uipropall.
   Qed.
 
   Lemma Own_Upd_set
         (r1: Σ) B
-        (UPD: URA.updatable_set r1 B)
+        (UPD: r1 ~~>: B)
     :
       (Own r1) ⊢ (#=> (∃ b, ⌜B b⌝ ∗ (Own b)))
   .
   Proof.
     cut (Entails (Own r1) (Upd (Ex (fun b => Sepconj (Pure (B b)) (Own b))))); ss.
-    uipropall. i. red in H. des. subst.
-    exploit (UPD (ctx0 ⋅ ctx)).
-    { rewrite URA.add_assoc. eauto. }
-    i. des. exists (b ⋅ ctx0). split.
-    { rewrite <- URA.add_assoc. eauto. }
-    { exists b. uipropall. esplits; [|apply IN|reflexivity].
-      eapply URA.add_comm. }
+    uipropall. i. red in H. des. rewrite H in H0.
+    exploit (UPD 0 (Some (z ⋅ ctx))).
+    { simpl. apply cmra_valid_validN. rewrite (assoc op). done. }
+    i. des. exists (y ⋅ z). split.
+    { apply cmra_discrete_valid in x1.  rewrite -(assoc op). eauto. }
+    { exists y. uipropall. esplits; [|auto|reflexivity].
+      eapply (comm op). }
   Qed.
 
   Lemma Own_Upd
         (r1 r2: Σ)
-        (UPD: URA.updatable r1 r2)
+        (UPD: r1 ~~> r2)
     :
       (Own r1) ⊢ (#=> (Own r2))
   .
@@ -452,7 +430,7 @@ Section ILEMMAS.
 
   Lemma Own_extends
         (a b: Σ)
-        (EXT: URA.extends a b)
+        (EXT: a ≼ b)
     :
       Own b ⊢ Own a
   .
@@ -460,65 +438,39 @@ Section ILEMMAS.
     red. uipropall. ii. etrans; eauto.
   Qed.
 
-  Lemma Own_persistently (r : Σ) : Own r ⊢ <pers> Own (URA.core r).
+  Lemma Own_persistently (r : Σ) : Own r ⊢ <pers> Own (core r).
   Proof.
-    uipropall. i. rr; uipropall. apply URA.extends_core. ss.
+    uipropall. i. rr; uipropall. apply cmra_core_mono. ss.
   Qed.
 
-  Lemma OwnM_persistently {M : URA.t} `{@GRA.inG M Σ} (r : M) : OwnM r ⊢ <pers> OwnM (URA.core r).
+  Lemma OwnM_persistently {M : ucmra} `{@GRA.inG M Σ} (r : M) : OwnM r ⊢ <pers> OwnM (core r).
   Proof.
     unfold OwnM. rewrite GRA.embed_core. apply Own_persistently.
   Qed.
 
-  Lemma OwnM_unit {M : URA.t} `{@GRA.inG M Σ} : ⊢ OwnM ε.
+  Lemma OwnM_unit {M : ucmra} `{@GRA.inG M Σ} : ⊢ OwnM ε.
   Proof.
-    Local Transparent GRA.to_URA.
     rr; uipropall. i. rr; uipropall. rr. exists r.
-    rewrite GRA.embed_unit. rewrite URA.unit_idl. ss.
+    rewrite GRA.embed_unit. rewrite left_id. ss.
   Qed.
 
-  Lemma OwnM_Upd_set (M: URA.t) `{@GRA.inG M Σ}
+  Lemma OwnM_Upd_set (M: ucmra) `{IN: @GRA.inG M Σ}
         (r1: M) B
-        (UPD: URA.updatable_set r1 B)
+        (UPD: r1 ~~>: B)
     :
       (OwnM r1) ⊢ (#=> (∃ b, ⌜B b⌝ ∗ (OwnM b)))
   .
   Proof.
-    assert (UPDM: URA.updatable_set
-                    (GRA.embed r1)
-                    (fun r => exists m, r = GRA.embed m /\ B m)).
-    { red. i. red in UPD.
-      unshelve hexploit UPD.
-      { eapply (@eq_rect URA.t (Σ (@GRA.inG_id _ _ H)) (@URA.car)).
-        { eapply (ctx (@GRA.inG_id _ _ H)). }
-        { symmetry. eapply (@GRA.inG_prf _ _ H). }
-      }
-      Local Transparent GRA.to_URA.
-      { ur in WF. ss. specialize (WF GRA.inG_id).
-        destruct H. subst. ss.
-        unfold GRA.embed in WF. ss.
-        replace (PeanoNat.Nat.eq_dec inG_id inG_id)
-          with (@left (inG_id = inG_id) (inG_id <> inG_id) eq_refl) in WF; ss.
-        { des_ifs. repeat f_equal. eapply proof_irrelevance. }
-      }
-      i. des. exists (GRA.embed b). esplits; eauto.
-      ur. Local Transparent GRA.to_URA. ss.
-      i. unfold GRA.embed. des_ifs.
-      { ss. unfold PCM.GRA.cast_ra. destruct  H. subst. ss. }
-      { ur in WF. specialize (WF k). rewrite URA.unit_idl.
-        eapply URA.wf_mon. rewrite URA.add_comm. eauto.
-      }
-    }
     iIntros "H".
     iPoseProof (Own_Upd_set with "H") as "> H".
-    { eapply UPDM. }
-    iDestruct "H" as (b) "[% H1]". des. subst.
+    { eapply GRA.embed_updatable_set. apply UPD. }
+    iDestruct "H" as (b) "[%Hm H1]". destruct Hm as [m [? ?]]. subst.
     iModIntro. iExists m. iFrame. ss.
   Qed.
 
-  Lemma OwnM_Upd (M: URA.t) `{@GRA.inG M Σ}
+  Lemma OwnM_Upd (M: ucmra) `{@GRA.inG M Σ}
         (r1 r2: M)
-        (UPD: URA.updatable r1 r2)
+        (UPD: r1 ~~> r2)
     :
       (OwnM r1) ⊢ (#=> (OwnM r2))
   .
@@ -531,26 +483,27 @@ Section ILEMMAS.
     iPure "H0" as Hs. subst. iApply "H1".
   Qed.
 
-  Lemma OwnM_extends (M: URA.t) `{@GRA.inG M Σ}
+  Lemma OwnM_extends (M: ucmra) `{@GRA.inG M Σ}
         (a b: M)
-        (EXT: URA.extends a b)
+        (EXT: a ≼ b)
     :
       OwnM b ⊢ OwnM a
   .
   Proof.
-    red. unfold OwnM. uipropall. i. unfold URA.extends in *.
-    des. subst. rewrite <- GRA.embed_add.
-    rewrite <- URA.add_assoc. eauto.
+    red. unfold OwnM. uipropall. i. unfold included in *.
+    des. setoid_rewrite H0. setoid_rewrite EXT.
+    eexists. rewrite -GRA.embed_add.
+    rewrite -(assoc op). eauto.
   Qed.
 
-  Lemma IUpd_unfold I P
+  Lemma IUpd_unfold (I P : iProp)
     :
     #=(I)=> P ⊢ (I -∗ #=> (I ∗ P)).
   Proof.
     reflexivity.
   Qed.
 
-  Lemma IUpd_fold I P
+  Lemma IUpd_fold (I P : iProp)
     :
     (I -∗ #=> (I ∗ P)) ⊢ #=(I)=> P.
   Proof.
@@ -613,7 +566,7 @@ Section ILEMMAS.
   Qed.
 End ILEMMAS.
 
-Global Instance upd_elim_iupd `{GRA.t} I P Q
+Global Instance upd_elim_iupd `{Σ : GRA.t} (I P Q : iProp Σ)
        `{ElimModal _ True false false (#=(I)=> P) P Q R}
   :
   ElimModal True false false (#=> P) P Q R.
@@ -622,7 +575,7 @@ Proof.
   iPoseProof (Upd_IUpd with "H0") as "> H0". iApply "H1". auto.
 Qed.
 
-Global Instance iupd_elim_upd `{GRA.t} I P Q b
+Global Instance iupd_elim_upd `{Σ : GRA.t} (I P Q : iProp Σ) b
   :
   ElimModal True b false (#=> P) P (#=(I)=> Q) (#=(I)=> Q).
 Proof.
@@ -638,7 +591,7 @@ Proof.
   }
 Qed.
 
-Global Instance subiprop_elim_upd `{GRA.t} I J P Q b
+Global Instance subiprop_elim_upd `{Σ : GRA.t} (I J P Q : iProp Σ) b
   :
   ElimModal True b false ((SubIProp I J) ∗ #=(I)=> P) P (#=(J)=> Q) (#=(J)=> Q).
 Proof.
@@ -657,13 +610,14 @@ Tactic Notation "iOwnWf" constr(H) :=
 Tactic Notation "iOwnWf" constr(H) "as" ident(WF) :=
   iOwnWf' H;
   match goal with
-  | H0: @URA.wf _ _ |- _ => rename H0 into WF
+  | H0: @valid _ _ _ |- _ => rename H0 into WF
   end
 .
 
 Section AUX.
 
   Context {Σ: GRA.t}.
+  Notation iProp := (iProp Σ).
 
   Fixpoint sep_conjs (Ps : nat -> iProp) (n : nat) : iProp :=
     match n with
