src/simulation/ThreadsURA.v
@@ -1,20 +1,22 @@
 From sflib Require Import sflib.
 Require Import Coq.Classes.RelationClasses.
+From iris.algebra Require Import cmra updates functions lib.excl_auth.
+
 From Fairness Require Import Axioms NatStructsLarge.
-From Fairness Require Import PCMLarge.
+From Fairness Require Import PCM.
 From Fairness Require Import Mod.
 
 Set Implicit Arguments.
 
-(* Definition _thsRA {A: Type}: URA.t := Auth.t (Excl.t A). *)
-Global Instance thsRA {A: Type}: URA.t := (thread_id ==> Auth.t (Excl.t A))%ra.
+(* Definition _thsRA {A: Type}: ucmra := Auth.t (Excl.t A). *)
+Definition thsRA {A: Type}: ucmra := (thread_id ==> (excl_authUR $ leibnizO A))%ra.
 (* Compute (URA.car (t:=_thsRA)). *)
-(* Global Instance thsRA {A: Type}: URA.t := Auth.t (@_thsRA A). *)
+(* Global Instance thsRA {A: Type}: ucmra := Auth.t (@_thsRA A). *)
 
 Section THHAS.
 
-  Definition ae_white {A} (a: A) := @Auth.white (Excl.t A) (Some a).
-  Definition ae_black {A} (a: A) := @Auth.black (Excl.t A) (Some a).
+  Definition ae_white {A} (a: A) := ◯E (a : leibnizO A).
+  Definition ae_black {A} (a: A) := ●E (a : leibnizO A).
 
   Definition th_has {A: Type} (tid: thread_id) (a: A): (@thsRA A) :=
     fun _tid => if (tid_dec _tid tid) then ae_white a else ε.
@@ -33,17 +35,9 @@ Section THHAS.
   Proof. i. rewrite unfold_th_has. des_ifs. Qed.
 
   Lemma th_has_disj {A: Type}: forall tid0 tid1 (a0 a1: A),
-      URA.wf (th_has tid0 a0 ⋅ th_has tid1 a1) -> tid0 <> tid1.
-  Proof. ii. do 2 ur in H. clarify. specialize (H tid1). rewrite !th_has_hit in H. ss. ur in H. ss. Qed.
+      ✓ (th_has tid0 a0 ⋅ th_has tid1 a1) -> tid0 <> tid1.
+  Proof. ii. clarify. specialize (H tid1). rewrite discrete_fun_lookup_op !th_has_hit in H. ss. eapply excl_auth_frag_op_valid,H. Qed.
 
 End THHAS.
 Notation "tid |-> a" := (th_has tid a) (at level 20).
 Global Opaque th_has.
-
-(* black + delta --> new_black *)
-Definition add_delta_to_black `{M: URA.t} (b: Auth.t M) (w: Auth.t _): Auth.t _ :=
-  match b, w with
-  | Auth.excl e _, Auth.frag f1 => Auth.black (e ⋅ f1)
-  | _, _ => Auth.boom
-  end
-.
